src/natural_deduction.lean
@@ -1,4 +1,4 @@
-import form
+import formula
 
 variable {vars : Type}
 
@@ -54,3 +54,5 @@ begin
     simp
   }
 end
+
+#lint
